Model/Decode.v
@@ -132,6 +132,7 @@ Module i8051_PARSER.
   Definition direct := (field 8) @ ((fun r => Direct_op (@Word.repr 7 r)) : _ -> result_m operand_t).
   Definition immediate := (field 8) @ ((fun r => Imm_op (@Word.repr 7 r)) : _ -> result_m operand_t).
 
+  Definition immediate_16 := (field 8) @ ((fun r => Imm16_op (@Word.repr 15 r)) : _ -> result_m operand_t).
   Definition bit_address := (field 8) @ ((fun r => Bit_op (bit_addr (@Word.repr 7 r))) : _ -> result_m operand_t).
   Definition byte := (field 8) @ (@Word.repr 7 : _ -> result_m byte_t).
  (* Definition halfword := (field 16) @ (@Word.repr 15 : _ -> result_m half_t).
@@ -180,17 +181,19 @@ Module i8051_PARSER.
   Definition ANL_p := arith_p_with_direct ANL "0101".
   Definition ADD_p := arith_p ADD "0010".
 
-  Definition bitwise_p op := "1101" $$ (
+  Definition bitwise_p pre op := pre $$ (
                              bits "0011" @ (fun _ => op (Bit_op Alias.C) %% instruction_t)
                                     |+| "0010"  $$ bit_address @ (fun i => CLR i %% instruction_t)).
-  Definition SETB_p := bitwise_p SETB.
+  Definition SETB_p := bitwise_p "1101" SETB.
   Definition CLR_p := bits "11100100" @ (fun _ => CLR Acc_op %% instruction_t)
-                           |+| bitwise_p CLR.
+                           |+| bitwise_p "1100" CLR.
   Definition NOP_p := bits "00000000" @ (fun _ =>  NOP %% instruction_t).
   (* Now glue all of the individual instruction parsers together into 
      one big parser. *)
+  Definition LJMP_p := "00000010" $$ immediate_16 @ (fun a => LJMP a %%instruction_t).
+  Definition JMP_p := bits "01110011" @ (fun _ => JMP %% instruction_t).
   Definition instrs : list (parser instruction_t) :=
-    ANL_p::ADD_p::nil.
+    JMP_p::SETB_p::CLR_p::LJMP_p::NOP_p::ANL_p::ADD_p::nil.
 
   Fixpoint list2pair_t (l: list result) :=
     match l with
