Verif/VerifierDFA.v
@@ -1,0 +1,184 @@
+(* Copyright (c) 2011. Greg Morrisett, Gang Tan, Joseph Tassarotti, 
+   Jean-Baptiste Tristan, and Edward Gan.
+
+   This file is part of RockSalt.
+
+   This file is free software; you can redistribute it and/or
+   modify it under the terms of the GNU General Public License as
+   published by the Free Software Foundation; either version 2 of
+   the License, or (at your option) any later version.
+*)
+
+
+(** VerifierDFA.v:  
+    This file contains definitions of the parsers used to build the DFAs
+    used in FastVerifier.
+*)
+Add LoadPath "../Model".
+Require Import Coqlib.
+Require Import Parser.
+Require Import Ascii.
+Require Import String.
+Require Import List.
+Require Import Bits.
+Require Import Hex.
+Require Import Decode.
+Require Import Eqdep.
+Require Import Int32.
+Unset Automatic Introduction.
+Set Implicit Arguments.
+Open Scope char_scope.
+Require ExtrOcamlString.
+Require ExtrOcamlNatBigInt.
+Require ExtrOcamlNatInt.
+Import i8051_PARSER_ARG.
+Import i8051_PARSER.
+Import i8051_BASE_PARSER.
+
+Require Import i8051Syntax.
+
+(* In NaCl, ChunkSize is either 16 or 32 *)
+Definition logChunkSize := 5%nat.
+Definition chunkSize := two_power_nat logChunkSize.
+Notation int8_of_nat n := (@repr 7 (Z_of_nat n)).
+Definition safeMask := shl (Word.mone 7) (int8_of_nat logChunkSize).
+
+Fixpoint int2bools_aux (bs : Z -> bool) (n: nat) : list bool :=
+  match n with
+    | O => bs 0 :: nil
+    | S n' => bs (Z_of_nat n) :: int2bools_aux bs n'
+  end.
+
+Definition int_to_bools {s} (x: Word.int s) : list bool :=
+  int2bools_aux (Word.bits_of_Z (s+1) (Word.unsigned x)) s.
+
+Definition nat2bools(n:nat) : list bool := 
+  let bs := Word.bits_of_Z 8 (Z_of_nat n) in
+    (bs 7)::(bs 6)::(bs 5)::(bs 4)::(bs 3)::(bs 2)::(bs 1)::(bs 0)::nil.
+
+Definition make_dfa t (p:parser t) := build_dfa 256 nat2bools 400 (par2rec p).
+Implicit Arguments make_dfa [t].
+
+
+
+Definition non_cflow_instrs : list (parser instruction_t) := 
+    SETB_p::CLR_p::NOP_p::ANL_p::ADD_p::nil.
+
+
+
+(** The list of valid prefix and instruction parsers for non-control-flow
+    operations. *)
+
+Definition non_cflow_parser := alts non_cflow_instrs.
+
+(* Direct jumps. Destinations will be checked to see if 
+   they are known, valid starts of instructions. *)
+
+(* We only want to allow "near" jumps to direct, relative offsets *)
+
+Definition dir_cflow : list (parser instruction_t) :=
+ LJMP_p :: JMP_p ::nil. (* dir_near_JMP_p :: dir_near_Jcc_p :: dir_near_CALL_p :: nil.*)
+Import i8051Syntax.
+Lemma register_to_Z_identity1: forall r, Z_to_register (register_to_Z r) = r.
+Proof. destruct r; auto.
+Qed. 
+
+Definition register_to_bools (r: register) := 
+  let bs := Word.bits_of_Z 3 (register_to_Z r) in
+    (bs 2) :: (bs 1) :: (bs 0) :: nil.
+
+Fixpoint bitslist (bs: list bool) : parser unit_t :=
+  match bs with
+    | nil => Eps_p
+    | b::bs' => Cat_p (Char_p b) (bitslist bs') @ (fun _ => tt %% unit_t)
+  end.
+
+Fixpoint bitslist' (bs: list bool) : string :=
+  match bs with
+    | nil => EmptyString
+    | true::bs' => append "1" (bitslist' bs')
+    | false::bs' => append "0" (bitslist' bs')
+  end.
+
+Definition b8 := true::false::false::false::nil.
+Definition b3 := false::false::true::true::nil.
+Definition be := true::true::true::false::nil.
+Definition b0 := false::false::false::false::nil.
+Definition bf := true::true::true::true::nil.
+
+Definition mybits := b8 ++ b3 ++ be ++ b0 ++ be ++ b0 ++ bf ++ bf ++ be ++ b0.
+
+
+(* These are akin to the NaCl "pseudo-instruction" nacljmp. We will
+   check if the jump destination is appropriately masked by the
+   preceding AND *)
+
+  Fixpoint parseloop ps bytes := 
+    match bytes with 
+      | nil => None
+      | b::bs => match Decode.i8051_PARSER.parse_byte ps b with 
+                   | (ps', nil) => parseloop ps' bs
+                     (* JGM: FIX!  What to do with prefix? *)
+                   | (ps',(LJMP  (Imm_op disp) )::_) => 
+                     match bs with 
+                       | nil => Some disp
+                       | _ => None
+                     end
+                   | (ps', _) => None
+                 end
+    end.
+
+(** Next, we define a boolean-valued test that tells whether an instruction
+    is a valid non-control-flow instruction.  We should have the property
+    that the [non_cflow_parser] only builds instructions that satisfy this
+    predicate (as shown below.)  Furthermore, we should be able to argue
+    that for each of these instructions, the NaCL SFI invariants are preserved. 
+*)
+Definition no_imm_op(op1:operand) : bool := 
+  match op1 with 
+    | Imm_op _ => false
+    | _ => true
+  end.
+
+
+Definition no_prefix (p : prefix) : bool :=  true.
+
+(** We rule out JMPs and CALLs that are far (i.e., not near), that
+    are absolute instead of relative, that don't have an immediate
+    operand, or that have a selector. *)
+Definition dir_cflow_instr (pre:prefix) (ins: instr) : bool :=
+  match ins with
+    | LJMP (Imm_op _)  => true
+    | _ => false
+  end.
+
+(** This predicate is defined on a pair of prefixes and instructions and
+    captures the legal masked indirect jumps. *)
+Definition nacljmp_mask_instr (pfx1:prefix) (ins1:instr) (pfx2:prefix) (ins2:instr) :=
+  no_prefix pfx1 && no_prefix pfx2 && 
+  match ins1 with
+    | ANL (Reg_op r1) (Imm_op wd) => 
+      zeq (Word.signed wd) (Word.signed safeMask) &&
+      (if register_eq_dec r1 r1 then false else true)
+    | _ => false
+  end.
+Definition nacl_MASK_p : parser (pair_t instruction_t instruction_t):=
+  let imMask := (Imm_op (Word.repr hF0)) in
+  ( bits ("01010100"++"11110000") @ (fun _ => ANL Acc_op imMask %% instruction_t))
+    $ (("01010011") $$ bitslist' (int_to_bools (@Word.repr 7 Alias.DPL)) $$ bits "11110000" @ (fun _ => ANL (Direct_op (Word.repr Alias.DPL)) imMask %% instruction_t)).
+
+Definition nacl_JMP_p  :=
+  JMP_p.
+  
+Definition nacljmp_p  :
+  parser (pair_t (pair_t instruction_t instruction_t) instruction_t) :=
+    nacl_MASK_p $ (nacl_JMP_p).
+Definition nacljmp_mask :
+  list (parser (pair_t (pair_t instruction_t instruction_t) instruction_t))
+  := nacljmp_p :: nil.
+ 
+
+Definition dfas := (make_dfa non_cflow_parser, make_dfa (alts dir_cflow), make_dfa (alts nacljmp_mask)).
+(* Extraction "tables.ml" dfas.*)
+
+
